fstar/MLS.TreeSync.API.Types.fst
@@ -1,12 +1,13 @@
 module MLS.TreeSync.API.Types
 
 open Comparse
+open MLS.NetworkTypes
 open MLS.TreeSync.NetworkTypes
 open MLS.TreeSync.Level0.Types
 
 (** TreeSync state and accessors *)
 type treesync_state (bytes:Type0) {|bytes_like bytes|} (tkt:treekem_types bytes) = {
-  group_id: bytes;
+  group_id: mls_bytes bytes;
   levels: nat;
   tree: treesync bytes tkt levels 0;
   version: nat;
