fstar/MLS.TreeSync.IntegrityCheck.fst
@@ -56,7 +56,7 @@ let check_signature #bytes #cb #tkt lp group_id =
       group_id = (match lp.data.source with | LNS_commit () | LNS_update () -> group_id | _ -> ());
     } <: leaf_node_tbs_nt bytes tkt) in
     let leaf_package_bytes: bytes = serialize (leaf_node_tbs_nt bytes _) tbs in
-    if not (length leaf_package_bytes < pow2 30 && sign_with_label_pre #bytes "LeafNodeTBS" leaf_package_bytes) then error "check_signature: tbs too long"
+    if not (length leaf_package_bytes < pow2 30 && sign_with_label_pre #bytes "LeafNodeTBS" (length #bytes leaf_package_bytes)) then error "check_signature: tbs too long"
     else (
       if verify_with_label #bytes lp.data.signature_key "LeafNodeTBS" leaf_package_bytes lp.signature then
         return None
@@ -125,12 +125,20 @@ let check_internal_node #bytes #cb #tkt #l #i t =
   | None -> return IE_Good
   | Some np -> (
     parent_hash_from_left_ok <-- (
-      computed_parent_hash <-- compute_parent_hash np.content np.parent_hash (un_add right np.unmerged_leaves);
-      return (has_child_with_parent_hash left computed_parent_hash)
+      if not (compute_parent_hash_pre np.content (length #bytes np.parent_hash) (un_add right np.unmerged_leaves)) then
+        error "check_internal_node: parent hash precondition not verified"
+      else (
+        let computed_parent_hash = compute_parent_hash np.content np.parent_hash (un_add right np.unmerged_leaves) in
+        return (has_child_with_parent_hash left computed_parent_hash)
+      )
     );
     parent_hash_from_right_ok <-- (
-      computed_parent_hash <-- compute_parent_hash np.content np.parent_hash (un_add left np.unmerged_leaves);
-      return (has_child_with_parent_hash right computed_parent_hash)
+      if not (compute_parent_hash_pre np.content (length #bytes np.parent_hash) (un_add left np.unmerged_leaves)) then
+        error "check_internal_node: parent hash precondition not verified"
+      else (
+        let computed_parent_hash = compute_parent_hash np.content np.parent_hash (un_add left np.unmerged_leaves) in
+        return (has_child_with_parent_hash right computed_parent_hash)
+      )
     );
     if (parent_hash_from_left_ok || parent_hash_from_right_ok) then
       return IE_Good
