fstar/MLS.TreeSync.Level0.fst
@@ -7,39 +7,49 @@ open MLS.TreeSync.Level0.Types
 open MLS.Tree
 open MLS.TreeCommon
 open MLS.TreeSync.ParentHash
-open MLS.Result
 
 #set-options "--fuel 1 --ifuel 1"
 
 (*** Tree operations ***)
 
-val tree_add: #bytes:Type0 -> {|bytes_like bytes|} -> #tkt:treekem_types bytes -> #l:nat -> #i:tree_index l -> treesync bytes tkt l i -> li:leaf_index l i -> leaf_node_nt bytes tkt -> result (treesync bytes tkt l i)
+val tree_add_pre: #bytes:Type0 -> {|bytes_like bytes|} -> #tkt:treekem_types bytes -> #l:nat -> #i:tree_index l -> treesync bytes tkt l i -> li:leaf_index l i -> bool
+let rec tree_add_pre #bytes #bl #tkt #l #i t li =
+  match t with
+  | TLeaf _ -> true
+  | TNode opt_content left right ->
+    (if is_left_leaf li then tree_add_pre left li else tree_add_pre right li) && (
+    match opt_content with
+    | None -> true
+    | Some content -> li < pow2 32 && bytes_length #bytes (ps_nat_lbytes 4) (insert_sorted li content.unmerged_leaves) < pow2 30
+    )
+
+val tree_add: #bytes:Type0 -> {|bytes_like bytes|} -> #tkt:treekem_types bytes -> #l:nat -> #i:tree_index l -> t:treesync bytes tkt l i -> li:leaf_index l i -> leaf_node_nt bytes tkt -> Pure (treesync bytes tkt l i)
+  (requires tree_add_pre t li) (ensures fun _ -> True)
 let rec tree_add #bytes #bl #tkt #l #i t li lp =
   match t with
-  | TLeaf _ -> return (TLeaf (Some lp))
+  | TLeaf _ -> TLeaf (Some lp)
   | TNode opt_content left right -> (
-    new_opt_content <-- (
+    let new_opt_content = (
       match opt_content with
-      | None -> return None
-      | Some content -> (
-        if not (li < pow2 32) then
-          error ""
-        else if not (bytes_length #bytes (ps_nat_lbytes 4) (insert_sorted li content.unmerged_leaves) < pow2 30) then
-          error ""
-        else
-          return (Some ({content with unmerged_leaves = insert_sorted li content.unmerged_leaves}))
-      )
-    );
+      | None -> None
+      | Some content -> Some ({content with unmerged_leaves = insert_sorted li content.unmerged_leaves})
+    ) in
     if is_left_leaf li then (
-      new_left <-- (tree_add left li lp);
-      return (TNode new_opt_content new_left right)
+      TNode new_opt_content (tree_add left li lp) right
     ) else (
-      new_right <-- (tree_add right li lp);
-      return (TNode new_opt_content left new_right)
+      TNode new_opt_content left (tree_add right li lp)
     )
   )
 
-val compute_new_np_and_ph: #bytes:Type0 -> {|crypto_bytes bytes|} -> #tkt:treekem_types bytes -> #l:nat -> #i:tree_index l -> option (tkt.node_content) -> treesync bytes tkt l i -> mls_bytes bytes -> result (option (parent_node_nt bytes tkt) & mls_bytes bytes)
+val compute_new_np_and_ph_pre: #bytes:Type0 -> {|crypto_bytes bytes|} -> #tkt:treekem_types bytes -> #l:nat -> #i:tree_index l -> option (tkt.node_content) -> treesync bytes tkt l i -> mls_nat -> bool
+let compute_new_np_and_ph_pre #bytes #cb #tkt #l #i opt_ext_content sibling length_parent_parent_hash =
+  match opt_ext_content with
+  | None -> true
+  | Some ext_content -> compute_parent_hash_pre ext_content length_parent_parent_hash sibling
+
+val compute_new_np_and_ph: #bytes:Type0 -> {|crypto_bytes bytes|} -> #tkt:treekem_types bytes -> #l:nat -> #i:tree_index l -> opt_ext_content:option (tkt.node_content) -> sibling:treesync bytes tkt l i -> parent_parent_hash:mls_bytes bytes -> Pure (option (parent_node_nt bytes tkt) & mls_bytes bytes)
+  (requires compute_new_np_and_ph_pre opt_ext_content sibling (length #bytes parent_parent_hash))
+  (ensures fun _ -> True)
 let compute_new_np_and_ph #bytes #cb #tkt #l #i opt_ext_content sibling parent_parent_hash =
   let new_opt_content =
     match opt_ext_content with
@@ -50,24 +60,41 @@ let compute_new_np_and_ph #bytes #cb #tkt #l #i opt_ext_content sibling parent_p
     } <: parent_node_nt bytes tkt)
     | None -> None
   in
-  new_parent_parent_hash <-- (
+  let new_parent_parent_hash =
     match opt_ext_content with
-    | Some ext_content ->
-      compute_parent_hash ext_content parent_parent_hash sibling
-    | None -> return parent_parent_hash
-  );
-  return (new_opt_content, new_parent_parent_hash)
+    | Some ext_content -> compute_parent_hash ext_content parent_parent_hash sibling
+    | None -> parent_parent_hash
+  in
+  (new_opt_content, new_parent_parent_hash)
 
-val compute_leaf_parent_hash_from_external_path: #bytes:Type0 -> {|crypto_bytes bytes|} -> #tkt:treekem_types bytes -> #l:nat -> #i:tree_index l -> #li:leaf_index l i -> t:treesync bytes tkt l i -> external_pathsync bytes tkt l i li -> mls_bytes bytes -> result (mls_bytes bytes)
+val compute_leaf_parent_hash_from_external_path_pre: #bytes:Type0 -> {|crypto_bytes bytes|} -> #tkt:treekem_types bytes -> #l:nat -> #i:tree_index l -> #li:leaf_index l i -> treesync bytes tkt l i -> external_pathsync bytes tkt l i li -> mls_nat -> bool
+let rec compute_leaf_parent_hash_from_external_path_pre #bytes #cb #tkt #l #i #li t p length_parent_parent_hash =
+  match t, p with
+  | TLeaf _, PLeaf _ -> true
+  | TNode _ left right, PNode opt_ext_content p_next -> (
+    let (child, sibling) = get_child_sibling t li in
+    let new_length_parent_parent_hash =
+      match opt_ext_content with
+      | None -> length_parent_parent_hash
+      | Some _ -> hash_length #bytes
+    in
+    compute_new_np_and_ph_pre opt_ext_content sibling length_parent_parent_hash && (
+    if is_left_leaf li then
+      compute_leaf_parent_hash_from_external_path_pre left p_next new_length_parent_parent_hash
+    else
+      compute_leaf_parent_hash_from_external_path_pre right p_next new_length_parent_parent_hash
+    )
+  )
+
+val compute_leaf_parent_hash_from_external_path: #bytes:Type0 -> {|crypto_bytes bytes|} -> #tkt:treekem_types bytes -> #l:nat -> #i:tree_index l -> #li:leaf_index l i -> t:treesync bytes tkt l i -> p:external_pathsync bytes tkt l i li -> parent_parent_hash:mls_bytes bytes -> Pure (mls_bytes bytes)
+  (requires compute_leaf_parent_hash_from_external_path_pre t p (length #bytes parent_parent_hash))
+  (ensures fun _ -> True)
 let rec compute_leaf_parent_hash_from_external_path #bytes #cb #tkt #l #i #li t p parent_parent_hash =
   match t, p with
-  | TLeaf old_lp, PLeaf new_lp -> (
-    return parent_parent_hash
-  )
+  | TLeaf old_lp, PLeaf new_lp -> parent_parent_hash
   | TNode _ left right, PNode opt_ext_content p_next ->
     let (child, sibling) = get_child_sibling t li in
-    tmp <-- compute_new_np_and_ph opt_ext_content sibling parent_parent_hash;
-    let (_,  new_parent_parent_hash) = tmp in
+    let (_,  new_parent_parent_hash) = compute_new_np_and_ph opt_ext_content sibling parent_parent_hash in
     if is_left_leaf li then
       compute_leaf_parent_hash_from_external_path left p_next new_parent_parent_hash
     else
@@ -85,76 +112,105 @@ let rec set_external_path_leaf #bytes #cb #tkt #l #i #li p lp =
   | PLeaf _ -> PLeaf lp
   | PNode p_content p_next -> PNode p_content (set_external_path_leaf p_next lp)
 
-val get_leaf_package_tbs: #bytes:Type0 -> {|bytes_like bytes|} -> #tkt:treekem_types bytes -> leaf_node_data_nt bytes tkt -> bytes -> result bytes
+val get_leaf_package_tbs: #bytes:Type0 -> {|bytes_like bytes|} -> #tkt:treekem_types bytes -> leaf_node_data_nt bytes tkt -> mls_bytes bytes -> bytes
 let get_leaf_package_tbs #bytes #bl #tkt lp_data group_id =
-    if not (length group_id < pow2 30) then
-      internal_failure "sign_leaf: group_id is too long"
-    else (
-      let ln_tbs = ({
-        data = lp_data;
-        group_id = (match lp_data.source with |LNS_update () |LNS_commit() -> group_id |_ -> ());
-      } <: leaf_node_tbs_nt bytes tkt) in
-      return (serialize (leaf_node_tbs_nt bytes _) ln_tbs)
-    )
+  let ln_tbs = ({
+    data = lp_data;
+    group_id = (match lp_data.source with |LNS_update () |LNS_commit() -> group_id |_ -> ());
+  } <: leaf_node_tbs_nt bytes tkt) in
+  (serialize (leaf_node_tbs_nt bytes _) ln_tbs)
 
-val external_path_is_valid: #bytes:Type0 -> {|crypto_bytes bytes|} -> #tkt:treekem_types bytes -> #l:nat -> #i:tree_index l -> #li:leaf_index l i -> t:treesync bytes tkt l i -> external_pathsync bytes tkt l i li -> bytes -> result bool
+val external_path_is_valid: #bytes:Type0 -> {|crypto_bytes bytes|} -> #tkt:treekem_types bytes -> #l:nat -> #i:tree_index l -> #li:leaf_index l i -> t:treesync bytes tkt l i -> external_pathsync bytes tkt l i li -> mls_bytes bytes -> bool
 let external_path_is_valid #bytes #cb #tkt #l #i #li t p group_id =
   let old_lp = leaf_at t li in
   let new_lp = get_external_path_leaf p in
   //TODO: something stating that new_lp is related to old_lp
-  computed_parent_hash <-- compute_leaf_parent_hash_from_external_path t p root_parent_hash;
-  tbs <-- get_leaf_package_tbs new_lp.data group_id;
-  verification_key <-- (
-    if not (length #bytes new_lp.data.signature_key = sign_public_key_length #bytes) then
-      error "external_path_is_valid: verification key has wrong length"
-    else
-      return (new_lp.data.signature_key <: sign_public_key bytes)
-  );
-  signature <-- (
-    if not (length #bytes new_lp.signature = sign_signature_length #bytes) then
-      error "external_path_is_valid: signature has wrong length"
-    else
-      return (new_lp.signature <: sign_signature bytes)
-  );
-  if not (length tbs < pow2 30 && sign_with_label_pre #bytes "LeafNodeTBS" tbs) then error "external_path_is_valid: tbs too long"
-  else (
-    let signature_ok = verify_with_label verification_key "LeafNodeTBS" tbs signature in
-    let parent_hash_ok = (new_lp.data.source = LNS_commit () && (new_lp.data.parent_hash <: bytes) = computed_parent_hash) in
-    return (signature_ok && parent_hash_ok)
-  )
-
-val external_path_to_valid_external_path: #bytes:Type0 -> {|crypto_bytes bytes|} -> #tkt:treekem_types bytes -> #l:nat -> #i:tree_index l -> #li:leaf_index l i -> t:treesync bytes tkt l i -> external_pathsync bytes tkt l i li -> bytes -> sign_private_key bytes -> sign_nonce bytes -> result (external_pathsync bytes tkt l i li)
-let external_path_to_valid_external_path #bytes #cb #tkt #l #i #li t p group_id sign_key nonce =
-  computed_parent_hash <-- compute_leaf_parent_hash_from_external_path t p root_parent_hash;
-  let lp = get_external_path_leaf p in
-  if not (lp.data.source = LNS_commit ()) then
-    error "external_path_to_valid_external_path: source is not a commit"
-  else (
-    let new_lp_data = { lp.data with parent_hash = computed_parent_hash; } in
-    new_lp_tbs <-- get_leaf_package_tbs new_lp_data group_id;
-    if not (length new_lp_tbs < pow2 30 && sign_with_label_pre #bytes "LeafNodeTBS" new_lp_tbs) then error "external_path_to_valid_external_path: tbs too long"
-    else (
-      let new_signature = sign_with_label sign_key "LeafNodeTBS" new_lp_tbs nonce in
-      return (set_external_path_leaf p ({ data = new_lp_data; signature = new_signature }))
+  let signature_ok =
+    let tbs = get_leaf_package_tbs new_lp.data group_id in
+    (length tbs < pow2 30 && sign_with_label_pre #bytes "LeafNodeTBS" (length #bytes tbs)) &&
+    (length #bytes new_lp.data.signature_key = sign_public_key_length #bytes) &&
+    (length #bytes new_lp.signature = sign_signature_length #bytes) &&
+    verify_with_label #bytes new_lp.data.signature_key "LeafNodeTBS" tbs new_lp.signature
+  in
+  let parent_hash_ok =
+    compute_leaf_parent_hash_from_external_path_pre t p (length #bytes (root_parent_hash #bytes)) && (
+    let computed_parent_hash = compute_leaf_parent_hash_from_external_path t p root_parent_hash in
+    (new_lp.data.source = LNS_commit () && (new_lp.data.parent_hash <: bytes) = computed_parent_hash)
     )
+  in
+  (signature_ok && parent_hash_ok)
+
+val external_path_to_valid_external_path_pre: #bytes:Type0 -> {|crypto_bytes bytes|} -> #tkt:treekem_types bytes -> #l:nat -> #i:tree_index l -> #li:leaf_index l i -> t:treesync bytes tkt l i -> external_pathsync bytes tkt l i li -> mls_bytes bytes -> bool
+let external_path_to_valid_external_path_pre #bytes #cb #tkt #l #i #li t p group_id =
+  let lp = get_external_path_leaf p in
+  compute_leaf_parent_hash_from_external_path_pre t p (length #bytes (root_parent_hash #bytes)) &&
+  lp.data.source = LNS_update () && (
+    let tbs_length = ((prefixes_length #bytes ((ps_leaf_node_tbs_nt tkt).serialize ({data = lp.data; group_id;}))) + 2 + (hash_length #bytes - 1)) in
+    tbs_length < pow2 30 &&
+    sign_with_label_pre #bytes "LeafNodeTBS" tbs_length
   )
 
-val apply_external_path_aux: #bytes:Type0 -> {|crypto_bytes bytes|} -> #tkt:treekem_types bytes -> #l:nat -> #i:tree_index l -> #li:leaf_index l i -> t:treesync bytes tkt l i -> external_pathsync bytes tkt l i li -> mls_bytes bytes -> result (treesync bytes tkt l i)
-let rec apply_external_path_aux #bytes #cb #tkt #l #i #li t p parent_parent_hash =
+#push-options "--z3rlimit 50"
+val external_path_to_valid_external_path: #bytes:Type0 -> {|crypto_bytes bytes|} -> #tkt:treekem_types bytes -> #l:nat -> #i:tree_index l -> #li:leaf_index l i -> t:treesync bytes tkt l i -> p:external_pathsync bytes tkt l i li -> group_id:mls_bytes bytes -> sign_private_key bytes -> sign_nonce bytes -> Pure (external_pathsync bytes tkt l i li)
+  (requires external_path_to_valid_external_path_pre t p group_id)
+  (ensures fun _ -> True)
+let external_path_to_valid_external_path #bytes #cb #tkt #l #i #li t p group_id sign_key nonce =
+  let computed_parent_hash = compute_leaf_parent_hash_from_external_path t p root_parent_hash in
+  assume(length #bytes computed_parent_hash < hash_length #bytes);
+  let lp = get_external_path_leaf p in
+  let new_lp_data = { lp.data with source = LNS_commit (); parent_hash = computed_parent_hash; } in
+  ps_leaf_node_tbs_nt_length tkt ({data = lp.data; group_id;});
+  ps_leaf_node_tbs_nt_length tkt ({data = new_lp_data; group_id;});
+  ps_leaf_node_data_nt_length tkt lp.data;
+  ps_leaf_node_data_nt_length tkt new_lp_data;
+  ps_leaf_node_source_nt_length #bytes (LNS_commit ());
+  ps_leaf_node_source_nt_length #bytes (LNS_update ());
+  assert_norm(256 < pow2 14); //TODO do something about it
+  //This assert might be useful when the above lemma calls can be remove due to SMTPats (FStarLang/FStar#2609)
+  assert((prefixes_length #bytes ((ps_leaf_node_tbs_nt tkt).serialize ({data = new_lp_data; group_id;}))) <= ((prefixes_length #bytes ((ps_leaf_node_tbs_nt tkt).serialize ({data = lp.data; group_id;}))) + 2 + (hash_length #bytes - 1)));
+  let new_lp_tbs: bytes = serialize (leaf_node_tbs_nt bytes tkt) ({data = new_lp_data; group_id;}) in
+  let new_signature = sign_with_label sign_key "LeafNodeTBS" new_lp_tbs nonce in
+  set_external_path_leaf p ({ data = new_lp_data; signature = new_signature })
+#pop-options
+
+val apply_external_path_aux_pre: #bytes:Type0 -> {|crypto_bytes bytes|} -> #tkt:treekem_types bytes -> #l:nat -> #i:tree_index l -> #li:leaf_index l i -> t:treesync bytes tkt l i -> external_pathsync bytes tkt l i li -> mls_nat -> bool
+let rec apply_external_path_aux_pre #bytes #cb #tkt #l #i #li t p length_parent_parent_hash =
   match t, p with
-  | TLeaf _, PLeaf lp -> return (TLeaf (Some lp))
+  | TLeaf _, PLeaf _ -> true
   | TNode _ left right, PNode opt_ext_content p_next ->
     let (child, sibling) = get_child_sibling t li in
-    tmp <-- compute_new_np_and_ph opt_ext_content sibling parent_parent_hash;
-    let (new_opt_content, new_parent_parent_hash) = tmp in
-    if is_left_leaf li then (
-      new_left <-- (apply_external_path_aux left p_next new_parent_parent_hash);
-      return (TNode new_opt_content new_left right)
-    ) else (
-      new_right <-- (apply_external_path_aux right p_next new_parent_parent_hash);
-      return (TNode new_opt_content left new_right)
+    let new_length_parent_parent_hash =
+      match opt_ext_content with
+      | None -> length_parent_parent_hash
+      | Some _ -> hash_length #bytes
+    in
+    compute_new_np_and_ph_pre opt_ext_content sibling length_parent_parent_hash && (
+      if is_left_leaf li
+      then apply_external_path_aux_pre left p_next new_length_parent_parent_hash
+      else apply_external_path_aux_pre right p_next new_length_parent_parent_hash
     )
 
-val apply_external_path: #bytes:Type0 -> {|crypto_bytes bytes|} -> #tkt:treekem_types bytes -> #l:nat -> #i:tree_index l -> #li:leaf_index l i -> t:treesync bytes tkt l i -> external_pathsync bytes tkt l i li -> result (treesync bytes tkt l i)
+val apply_external_path_aux: #bytes:Type0 -> {|crypto_bytes bytes|} -> #tkt:treekem_types bytes -> #l:nat -> #i:tree_index l -> #li:leaf_index l i -> t:treesync bytes tkt l i -> p:external_pathsync bytes tkt l i li -> parent_parent_hash:mls_bytes bytes -> Pure (treesync bytes tkt l i)
+  (requires apply_external_path_aux_pre t p (length #bytes parent_parent_hash))
+  (ensures fun _ -> True)
+let rec apply_external_path_aux #bytes #cb #tkt #l #i #li t p parent_parent_hash =
+  match t, p with
+  | TLeaf _, PLeaf lp -> TLeaf (Some lp)
+  | TNode _ left right, PNode opt_ext_content p_next ->
+    let (child, sibling) = get_child_sibling t li in
+    let (new_opt_content, new_parent_parent_hash) = compute_new_np_and_ph opt_ext_content sibling parent_parent_hash in
+    if is_left_leaf li then (
+      TNode new_opt_content (apply_external_path_aux left p_next new_parent_parent_hash) right
+    ) else (
+      TNode new_opt_content left (apply_external_path_aux right p_next new_parent_parent_hash)
+    )
+
+val apply_external_path_pre: #bytes:Type0 -> {|crypto_bytes bytes|} -> #tkt:treekem_types bytes -> #l:nat -> #i:tree_index l -> #li:leaf_index l i -> t:treesync bytes tkt l i -> external_pathsync bytes tkt l i li -> bool
+let apply_external_path_pre #bytes #cb #tkt #l #i #li t p =
+  apply_external_path_aux_pre t p (length #bytes (root_parent_hash #bytes))
+
+val apply_external_path: #bytes:Type0 -> {|crypto_bytes bytes|} -> #tkt:treekem_types bytes -> #l:nat -> #i:tree_index l -> #li:leaf_index l i -> t:treesync bytes tkt l i -> p:external_pathsync bytes tkt l i li -> Pure (treesync bytes tkt l i)
+  (requires apply_external_path_pre t p)
+  (ensures fun _ -> True)
 let apply_external_path #bytes #cb #tkt #l #i #li t p =
   apply_external_path_aux t p root_parent_hash
