fstar/MLS.TreeSync.ParentHash.fst
@@ -19,6 +19,7 @@ type parent_hash_input_nt (bytes:Type0) {|bytes_like bytes|} (tkt:treekem_types 
 }
 
 %splice [ps_parent_hash_input_nt] (gen_parser (`parent_hash_input_nt))
+%splice [ps_parent_hash_input_nt_length] (gen_length_lemma (`parent_hash_input_nt))
 
 instance parseable_serializeable_parent_hash_input_nt (bytes:Type0) {|bytes_like bytes|} (tkt:treekem_types bytes): parseable_serializeable bytes (parent_hash_input_nt bytes tkt) =
   mk_parseable_serializeable (ps_parent_hash_input_nt tkt)
@@ -47,17 +48,25 @@ let rec un_add #bytes #bl #tkt #l #i t leaves =
     let new_right = un_add right leaves in
     TNode new_onp new_left new_right
 
-//Note: We could remove the `result` (i.e. prove that the hash input doesn't exceed pow2 61 + add precondition).
-val compute_parent_hash: #bytes:Type0 -> {|crypto_bytes bytes|} -> #tkt:treekem_types bytes -> #l:nat -> #i:tree_index l -> tkt.node_content -> mls_bytes bytes -> treesync bytes tkt l i -> result (mls_bytes bytes)
-let compute_parent_hash #bytes #cb #tkt #l #i kem_content parent_hash sibling =
-  original_sibling_tree_hash <-- tree_hash sibling;
+val compute_parent_hash_pre: #bytes:Type0 -> {|crypto_bytes bytes|} -> #tkt:treekem_types bytes -> #l:nat -> #i:tree_index l -> tkt.node_content -> mls_nat -> treesync bytes tkt l i -> bool
+let compute_parent_hash_pre #bytes #cb #tkt #l #i content parent_hash_length original_sibling =
+  tree_hash_pre original_sibling &&
+  prefixes_length (tkt.ps_node_content.serialize content) + 4 + parent_hash_length + 2 + hash_length #bytes < hash_max_input_length #bytes
+
+#push-options "--z3rlimit 50"
+val compute_parent_hash: #bytes:Type0 -> {|crypto_bytes bytes|} -> #tkt:treekem_types bytes -> #l:nat -> #i:tree_index l -> content:tkt.node_content -> parent_hash:mls_bytes bytes -> original_sibling:treesync bytes tkt l i{compute_parent_hash_pre content (length #bytes parent_hash) original_sibling} -> lbytes bytes (hash_length #bytes)
+let compute_parent_hash #bytes #cb #tkt #l #i content parent_hash original_sibling =
+  let original_sibling_tree_hash = tree_hash original_sibling in
   let hash_input = serialize #bytes (parent_hash_input_nt bytes tkt) ({
-    content = kem_content;
+    content;
     parent_hash = parent_hash;
     original_sibling_tree_hash;
   }) in
-  if not (length hash_input < hash_max_input_length #bytes) then error ""
-  else return (hash_hash #bytes hash_input <: mls_bytes bytes)
+  assert_norm(256 < pow2 14); //TODO
+  //TODO: remove next line when we have FStarLang/FStar#2609
+  ps_parent_hash_input_nt_length tkt ({content; parent_hash; original_sibling_tree_hash;});
+  hash_hash #bytes hash_input
+#pop-options
 
 val root_parent_hash: #bytes:Type0 -> {|bytes_like bytes|} -> mls_bytes bytes
 let root_parent_hash #bytes #bl = empty #bytes
