fstar/MLS.TreeSync.API.fst
@@ -2,6 +2,7 @@ module MLS.TreeSync.API
 
 open Comparse
 open MLS.Crypto
+open MLS.NetworkTypes
 open MLS.TreeSync.NetworkTypes
 open MLS.Tree
 open MLS.TreeCommon
@@ -10,7 +11,7 @@ open MLS.TreeSync.Level0
 open MLS.TreeSync.API.Types
 open MLS.Result
 
-val create: #bytes:Type0 -> {|bytes_like bytes|} -> #tkt:treekem_types bytes -> gid:bytes -> leaf_node_nt bytes tkt -> treesync_state bytes tkt
+val create: #bytes:Type0 -> {|bytes_like bytes|} -> #tkt:treekem_types bytes -> gid:mls_bytes bytes -> leaf_node_nt bytes tkt -> treesync_state bytes tkt
 let create #bytes #bl gid lp =
   {
     group_id = gid;
@@ -41,13 +42,17 @@ let add #bytes #bl #tkt st kp =
   lp <-- get_leaf_package_from_key_package kp;
   match find_empty_leaf st.tree with
   | Some i ->
-    new_tree <-- tree_add st.tree i lp;
-    return (state_update_tree st new_tree, (i <: nat))
+    if not (tree_add_pre st.tree i) then
+      error "add: tree_add_pre is false"
+    else
+      return (state_update_tree st (tree_add st.tree i lp), (i <: nat))
   | None ->
     let augmented_tree = add_one_level st.tree in
     let i = Some?.v (find_empty_leaf augmented_tree) in
-    new_tree <-- tree_add augmented_tree i lp;
-    return (state_update_tree st new_tree, (i <: nat))
+    if not (tree_add_pre augmented_tree i) then
+      error "add: tree_add_pre is false (after extension)"
+    else
+      return (state_update_tree st (tree_add augmented_tree i lp), (i <: nat))
 
 val update: #bytes:Type0 -> {|bytes_like bytes|} -> #tkt:treekem_types bytes -> st:treesync_state bytes tkt -> leaf_node_nt bytes tkt -> treesync_index st -> treesync_state bytes tkt
 let update #bytes #bl #tkt st lp i =
@@ -61,5 +66,7 @@ let remove #bytes #bl #tkt st i =
 
 val commit: #bytes:Type0 -> {|crypto_bytes bytes|} -> #tkt:treekem_types bytes -> st:treesync_state bytes tkt -> #li:treesync_index st -> external_pathsync bytes tkt st.levels 0 li -> result (treesync_state bytes tkt)
 let commit #bytes #cb #tkt st #li p =
-  new_tree <-- apply_external_path st.tree p;
-  return (state_update_tree st new_tree)
+  if not (apply_external_path_pre st.tree p) then
+    error "commit: bad precondition"
+  else
+    return (state_update_tree st (apply_external_path st.tree p))
