fstar/MLS.TreeSync.NetworkTypes.fst
@@ -65,6 +65,7 @@ type leaf_node_source_nt =
   | LNS_commit:      [@@@ with_num_tag 1 3] unit -> leaf_node_source_nt
 
 %splice [ps_leaf_node_source_nt] (gen_parser (`leaf_node_source_nt))
+%splice [ps_leaf_node_source_nt_length] (gen_length_lemma (`leaf_node_source_nt))
 
 /// struct {
 ///     ProtocolVersion versions<V>;
@@ -156,6 +157,7 @@ type leaf_node_data_nt (bytes:Type0) {|bytes_like bytes|} (tkt:treekem_types byt
 }
 
 %splice [ps_leaf_node_data_nt] (gen_parser (`leaf_node_data_nt))
+%splice [ps_leaf_node_data_nt_length] (gen_length_lemma (`leaf_node_data_nt))
 
 type leaf_node_nt (bytes:Type0) {|bytes_like bytes|} (tkt:treekem_types bytes) = {
   data: leaf_node_data_nt bytes tkt;
@@ -218,6 +220,7 @@ type leaf_node_tbs_nt (bytes:Type0) {|bytes_like bytes|} (tkt:treekem_types byte
 }
 
 %splice [ps_leaf_node_tbs_nt] (gen_parser (`leaf_node_tbs_nt))
+%splice [ps_leaf_node_tbs_nt_length] (gen_length_lemma (`leaf_node_tbs_nt))
 
 instance parseable_serializeable_leaf_node_tbs_nt (bytes:Type0) {|bytes_like bytes|} (tkt:treekem_types bytes): parseable_serializeable bytes (leaf_node_tbs_nt bytes tkt) = mk_parseable_serializeable (ps_leaf_node_tbs_nt tkt)
 
@@ -287,6 +290,7 @@ type node_type_nt =
   | NT_parent: [@@@ with_num_tag 1 2] unit -> node_type_nt
 
 %splice [ps_node_type_nt] (gen_parser (`node_type_nt))
+%splice [ps_node_type_nt_length] (gen_length_lemma (`node_type_nt))
 
 /// struct {
 ///     NodeType node_type;
